import Relation.Binary.PropositionalEquality as Eq
open Eq using (_≡_; refl)
open Eq.≡-Reasoning using (begin_; _≡⟨⟩_; _∎)

data ℕ : Set where
  zero : ℕ
  suc  : ℕ → ℕ
  
{-# BUILTIN NATURAL ℕ #-}

infixl 6  _+_  _∸_
infixl 7  _*_

_+_ : ℕ → ℕ → ℕ
zero + n = n
(suc m) + n = suc (m + n)

_*_ : ℕ → ℕ → ℕ
zero    * n  =  zero
(suc m) * n  =  n + (m * n)

_∸_ : ℕ → ℕ → ℕ
m     ∸ zero   =  m
zero  ∸ suc n  =  zero
suc m ∸ suc n  =  m ∸ n

_ : 2 + 3 ≡ 5
_ = refl

_^_ : ℕ → ℕ → ℕ
m ^ zero = suc zero
m ^ suc n = m * (m ^ n)
